First proof inspired by original: CH2B.4

Definitions/Combinators.v
@@ -3,6 +3,7 @@ Open Scope combinator_scope.
 
 Inductive combinator : Type := 
     B | C | K | W 
+    | Var (n : nat)
     | Apply (x y : combinator).
 
 Notation "a @ b" :=
