Definitions/Semantics.v
@@ -1,41 +1,82 @@
-From Definitions Require Export Combinators.
+From Definitions Require Export Combinators Properties.
 
 Create HintDb hclt.
 Ltac hauto := eauto with hclt.
 
 Reserved Notation "a ~> b" (at level 20).
-Inductive sstep : combinator -> combinator -> Prop :=
-| ExecB : forall x y z, (B @ x @ y @ z) ~> (x @ (y @ z))
-| ExecC : forall x y z, (C @ x @ y @ z) ~> (x @ z @ y)
-| ExecK : forall x y,   (K @ x @ y) ~> x
-| ExecW : forall x y,   (W @ x @ y) ~> (x @ y @ y)
-| ExecAppL : forall x x' y, x ~> x' -> (x @ y) ~> (x' @ y)
-| ExecAppR : forall x y y', y ~> y' -> (x @ y) ~> (x @ y')
-    where "a ~> b" := (sstep a b).
+Inductive step : combinator -> combinator -> Prop :=
+| StepB : forall x y z, (B @ x @ y @ z) ~> (x @ (y @ z))
+| StepC : forall x y z, (C @ x @ y @ z) ~> (x @ z @ y)
+| StepK : forall x y,   (K @ x @ y) ~> x
+| StepW : forall x y,   (W @ x @ y) ~> (x @ y @ y)
+| StepAppL : 
+    forall x x' y, 
+    x ~> x' -> 
+    (x @ y) ~> (x' @ y)
+| StepAppR : 
+    forall x y y',
+    y ~> y' -> 
+    (x @ y) ~> (x @ y')
+where "a ~> b" := (step a b).
 
-Hint Constructors sstep : hclt.
+Hint Constructors step : hclt.
+
+Reserved Notation "a ~>* b" (at level 21).
+Inductive multistep : combinator -> combinator -> Prop :=
+| step_none : forall c, c ~>* c
+| step_one : forall c c', c ~> c' -> c ~>* c'
+| step_multi : forall c c' c'', c ~> c' -> c' ~>* c'' -> c ~>* c''
+where "a ~>* b" := (multistep a b).
+
+Hint Constructors multistep : hclt.
+
+Theorem multistep_trans :
+    transitive multistep.
+Proof. unfold transitive. hauto. Qed.
+
+Hint Resolve multistep_trans : hclt.
 
 Inductive Q : combinator -> combinator -> Prop :=
 | Def2 : forall x y, x = y -> Q x y
-| Qlr : forall x y, x ~> y -> Q x y
-| Qrl : forall x y, y ~> x -> Q x y
-| Qstepl : forall x x' y, x ~> x' -> Q x' y -> Q x y
-| Qstepr : forall x y y', y ~> y' -> Q x y' -> Q x y
+| Qlr : forall x y, x ~>* y -> Q x y
+| Qrl : forall x y, y ~>* x -> Q x y
+| Qstepl : forall x x' y, x ~>* x' -> Q x' y -> Q x y
+| Qstepr : forall x y y', y ~>* y' -> Q x y' -> Q x y
 | Q_trans : forall x y z, Q x y -> Q y z -> Q x z. 
 
 Hint Constructors Q : hclt.
+
+Tactic Notation "step" "right" :=
+    solve [now constructor] || (eapply Qstepr; 
+    [eapply step_multi; repeat constructor; hauto |]).
+Tactic Notation "step" "left" :=
+    solve [now constructor] || (eapply Qstepl; 
+    [eapply step_multi; repeat constructor; hauto |]).
 
 (* Definition 3 *)
 Definition _I := W @ K.
 
 (* Remark *)
 Definition _S : combinator :=
-    B @ (B @ (B @ W) @ C) @ (B @ B).
+    B @ (B @ W) @ (B @ B @ C).
+
+Lemma mstep_app_r : forall x y z,
+    y ~>* z ->
+    (x @ y) ~>* (x @ z).
+Proof with hauto. intros; induction H... Qed.
+
+Lemma mstep_app_l : forall x y z,
+    x ~>* y ->
+    (x @ z) ~>* (y @ z).
+Proof with hauto. intros; induction H... Qed.
+
+Hint Resolve mstep_app_r : hclt.
+Hint Resolve mstep_app_l : hclt.
 
 Theorem Q_app_l : forall x y w,
     Q x y -> Q (w @ x) (w @ y).
 Proof with hauto.
-    intros. induction H... subst...
+    intros. induction H; subst...
 Qed.
 
 Theorem RuleB : forall x y z,
