Proofs/Part1/Ch1D.v
@@ -10,7 +10,6 @@ Theorem Q_sym:
     forall x y, Q x y -> Q y x.
 Proof with hauto. 
     intros; induction H...
-    Unshelve. exact B.
 Qed.
 
 (* Theorem 3 *)
@@ -23,15 +22,15 @@ Theorem Q_app_r :
     forall x y z,
     Q x y -> Q (x @ z) (y @ z).
 Proof with hauto.
-    intros; induction H...
-    subst...
+    intros; induction H; subst...
 Qed.
 
 (* Theorem 6 *)
-Require Export Coq.Classes.RelationClasses.
-Require Export Coq.Setoids.Setoid.
+Require Export Classes.RelationClasses.
+Require Export Setoids.Setoid.
+Require Export Classes.Morphisms.
 
-Instance Q_equiv : Equivalence Q.
+Instance: Equivalence Q.
 Proof.
   constructor.
     unfold Reflexive. apply Q_refl.
@@ -44,6 +43,11 @@ Add Parametric Relation : combinator Q
   symmetry proved by Q_sym
   transitivity proved by Q_trans
   as Q_setoid.
+
+Instance : Proper (eq ==> Q ==> Q) Apply.
+Proof with hauto.
+    intros x y eq x0 y0 H. subst...
+Qed.
 
 (* Theorem 7 *)
 Require Import List.
@@ -69,6 +73,46 @@ Proof.
     now inversion H0.
 Qed.
 
+Fixpoint sublist {A : Type} (l : list A) (i : nat) : list A :=
+    match i, l with
+    | O, _ => []
+    | S i', [] => []
+    | S i', h :: t =>
+        h :: sublist t i'
+    end.
+
+Lemma sublist_length : forall (A : Type) (l : list A),
+    sublist l (length l) = l.
+Proof.
+    induction l; simpl.
+        reflexivity.
+    now rewrite IHl.
+Qed.
+
+Lemma nth_eq_sublist_eq :
+    forall (A : Type) (l1 l2 : list A)
+           (n i : nat)
+           (d : A),
+    length l1 = length l2 ->
+    n < i ->
+    nth n l1 d = nth n l2 d ->
+    sublist l1 i = sublist l2 i.
+Admitted.
+
+Lemma nth_eq_list_eq :
+    forall (A : Type) (l1 l2 : list A)
+           (i : nat)
+           (d : A),
+    length l1 = length l2 ->
+    i < length l1 ->
+    nth i l1 d = nth i l2 d ->
+    l1 = l2.
+Proof.
+    intros.
+    pose proof (nth_eq_sublist_eq A l1 l2 i (length l1) d H H0 H1).
+    now rewrite sublist_length, H, sublist_length in H2.
+Qed.
+
 Theorem list_comb_app_inv :
     forall (Xl Dl : list combinator)
            (X D default : combinator)
@@ -79,25 +123,45 @@ Theorem list_comb_app_inv :
     i < length Xl ->
     nth i Xl default = nth i Dl default ->
     X = D.
-Abort.
+Proof.
+    intros.
+    pose proof (nth_eq_list_eq combinator Xl Dl i default H1 H2 H3).
+    subst. rewrite <- H in H0. now inversion H0.
+Qed.
 
 (* Theorem 9 *)
 Theorem id_x : forall x,
     Q (_I @ x) x.
 Proof. hauto. Qed.
 
-Corollary Schonfinkel_KSB :
-    Q B (_S @ (K @ _S) @ K).
+Corollary Schonfinkel_KSB : forall x y z,
+    Q (B @ x @ y @ z) (_S @ (K @ _S) @ K @ x @ y @ z).
+Proof.
+    intros. unfold _S.
+    step left.
+    repeat (step right).
+Qed.
+
+Corollary Schonfinkel_KSC : forall x y z,
+    Q (C @ x @ y @ z) (_S @ (B @ B @ _S) @ (K @ K) @ x @ y @ z).
+Proof.
+    intros. unfold _S.
+    step left.
+    do 14 (step right).
 Abort.
 
-Corollary Schonfinkel_KSC :
-    Q C (_S @ (B @ B @ _S) @ (K @ K)).
+Corollary Schonfinkel_KSW : forall x y,
+    Q (W @ x @ y) (_S @ _S @ (_S @ K) @ x @ y).
+Proof.
+    intros. unfold _S.
+    step left.
+    do 12 (step right).
 Abort.
 
-Corollary Schonfinkel_KSW :
-    Q W (_S @ _S @ (_S @ K)).
-Abort.
-
-Corollary Schonfinkel_KSI :
-    Q _I (_S @ K @ K).
-Abort.
+Corollary Schonfinkel_KSI : forall x,
+    Q (_I @ x) (_S @ K @ K @ x).
+Proof.
+    intros. unfold _I, _S.
+    step left. step left.
+    repeat step right.
+Qed.
