Proofs/Part1/Ch2B.v
@@ -1,32 +1,110 @@
 From Proofs Require Import Ch1D.
 
 (* Section 1 : The B Sequence *)
-Fixpoint B_seq (n : nat) : combinator :=
+Fixpoint Bseq (n : nat) : combinator :=
     match n with
     | 0 => _I
     | 1 => B
-    | S n' => B @ B @ B_seq n'
+    | S n' => B @ B @ Bseq n'
     end.
 
-Lemma B_seq_Sn : forall n,
+Lemma Bseq_Sn : forall n,
     1 <= n ->
-    B_seq (S n) = B @ B @ B_seq n.
+    Bseq (S n) = B @ B @ Bseq n.
 Proof. 
     intros. simpl. destruct n. inversion H.
     destruct n; simpl; reflexivity.
 Qed.
 
 (* Theorem 1 *)
-Theorem B_Sn_xyz__Bn_xyz :
+Theorem Bseq_Sn_xyz__Bseq_n_xyz :
     forall x y z n,
-    Q (B_seq (S n) @ x @ y @ z) (B_seq n @ x @ (y @ z)).
-Proof.
-    intros. destruct n.
-    - hauto.
-    - rewrite B_seq_Sn.
-        etransitivity.
-            apply Qlr. hauto.
-        etransitivity.
-            apply Qlr. hauto.
-        hauto. apply le_n_S, PeanoNat.Nat.le_0_l.
+    Q (Bseq (S n) @ x @ y @ z) (Bseq n @ x @ (y @ z)).
+Proof with hauto.
+    intros; destruct n...
 Qed.
+
+(* Theorem 2 *)
+(* Compute (Bseq (0 + 0), Bseq 0 @ Bseq 0).
+Compute (Bseq (0 + 1), Bseq 0 @ Bseq 1).
+Compute (Bseq (1 + 0), Bseq 1 @ Bseq 0).
+Compute (Bseq (1 + 1), Bseq 1 @ Bseq 1).
+
+Lemma Bseq_plus :
+    forall n m,
+    Q (Bseq (n + m)) (Bseq n @ Bseq m).
+Proof with hauto.
+    induction n; intros.
+    - repeat step right.
+    - change (S n + m) with (S (n + m)).
+      destruct (PeanoNat.Nat.le_ge_cases 1 n).
+      -- rewrite Bseq_Sn, Bseq_Sn, IHn.
+         step right. rewrite <- IHn. *)
+
+Theorem Bseq_nm_xyzm__Bseq_n_x_yzm :
+    forall (m n : nat) (x y z : combinator) (Zl : list combinator),
+    Some z = app_comb_list Zl ->
+    m = length Zl ->
+    Q (Bseq (n + m) @ x @ y @ z) (Bseq n @ x @ (y @ z)).
+Proof.
+    induction m as [| k IH]; intros.
+    - rewrite PeanoNat.Nat.add_0_r. symmetry in H0.
+      apply -> List.length_zero_iff_nil in H0. subst.
+      inversion H.
+    - destruct k.
+        now rewrite <- PeanoNat.Nat.add_comm, Bseq_Sn_xyz__Bseq_n_xyz.
+        rewrite <- PeanoNat.Nat.add_succ_comm.
+        change (S n + S k) with (S (n + S k)).
+        rewrite Bseq_Sn_xyz__Bseq_n_xyz.
+        rewrite <- PeanoNat.Nat.add_succ_comm.
+        change (S n + k) with (S (n + k)).
+Admitted.
+
+(* Theorem 3 *)
+Theorem Bseq_m_xyzm__x_yzm :
+    forall m x y z Zl,
+    Some z = app_comb_list Zl ->
+    m = length Zl ->
+    Q (Bseq m @ x @ y @ z) (x @ (y @ z)).
+Proof.
+    intros. pose proof (Bseq_nm_xyzm__Bseq_n_x_yzm m 0 x y z Zl H H0).
+    simpl in H1. transitivity (_I @ x @ (y @ z)).
+        assumption.
+    step left. step left. reflexivity.
+Qed.
+
+(* Theorem 4 *)
+Theorem X_nm__BmXn :
+    forall (m n : nat) (Xl : list combinator) (d : combinator),
+    1 <= n < length Xl ->
+    (forall n, Q (List.nth (S n) Xl d) (B @ (List.nth n Xl d))) ->
+    Q (List.nth (n + m) Xl d) (Bseq m @ (List.nth n Xl d)).
+Proof with hauto.
+    induction m; intros.
+    - simpl. step right. step right. rewrite PeanoNat.Nat.add_0_r...
+    - destruct m.
+        rewrite PeanoNat.Nat.add_comm...
+        remember (S m) as k.
+        rewrite <- PeanoNat.Nat.add_succ_comm.
+        change (S n + k) with (S (n + k)).
+        rewrite H0, IHm...
+        rewrite Bseq_Sn... subst. apply le_n_S, PeanoNat.Nat.le_0_l.
+Qed.
+
+(* Theorem 5 *)
+Theorem Bm_BnX__BmnX :
+    forall (n m : nat) (X : combinator),
+    Q (Bseq m @ (Bseq n @ X)) (Bseq (m + n) @ X).
+Proof with hauto.
+    induction n as [| n']; intros.
+    - rewrite PeanoNat.Nat.add_0_r...
+    - rewrite PeanoNat.Nat.add_comm. change (S n' + m) with (S (n' + m)).
+      destruct (PeanoNat.Nat.eq_dec n' 0).
+      -- subst. specialize (IHn' m X). 
+         rewrite PeanoNat.Nat.add_0_r in IHn'. simpl in IHn'.
+         destruct m. step left. step left. reflexivity.
+         rewrite Bseq_Sn with (n := 0 + S m).
+         step right. change (0 + S m) with (S m). rewrite <- IHn'.
+         simpl (Bseq 1).
+         assert (Q (_I @ X) X) by now step left. rewrite H. clear H.
+Admitted. (* Almost... *)
