Definitions/Properties.v
@@ -1,0 +1,13 @@
+Definition relation (X : Type) := X -> X -> Prop.
+
+Definition deterministic {X : Type} (R : relation X) :=
+  forall x y1 y2 : X, R x y1 -> R x y2 -> y1 = y2.
+
+Definition transitive {X : Type} (R : relation X) :=
+    forall a b c, R a b -> R b c -> R a b.
+
+Definition symmetric {X : Type} (R : relation X) :=
+    forall a b, R a b -> R b a.
+
+Definition reflexive {X : Type} (R : relation X) :=
+    forall a, R a a.
